theories/simplang/locations.v
@@ -4,7 +4,8 @@ From stdpp Require Import countable numbers gmap.
 (* partly adapted from lambda rust *)
 
 Definition block := positive.
-Record loc := mkloc { loc_chunk : block; loc_idx : Z }.
+Record loc := Loc { loc_chunk : block; loc_idx : Z }.
+Add Printing Constructor loc.
 
 Global Instance loc_eq_decision : EqDecision loc.
 Proof. solve_decision. Qed.
@@ -19,7 +20,7 @@ Program Instance loc_infinite : Infinite loc :=
 Next Obligation. intros []. done. Qed.
 
 Definition loc_add (l : loc) (off : Z) : loc :=
-  {| loc_chunk := loc_chunk l; loc_idx := loc_idx l + off|}.
+  Loc (loc_chunk l) (loc_idx l + off).
 
 Notation "l +ₗ off" :=
   (loc_add l off) (at level 50, left associativity) : stdpp_scope.
@@ -35,17 +36,17 @@ Proof. done. Qed.
 Global Instance loc_add_inj l : Inj eq eq (loc_add l).
 Proof. destruct l; rewrite /Inj /loc_add /=; intros; simplify_eq; lia. Qed.
 
-Lemma loc_eta l : (mkloc (loc_chunk l) (loc_idx l)) = l.
+Lemma loc_eta l : (Loc (loc_chunk l) (loc_idx l)) = l.
 Proof.  by destruct l. Qed.
-Lemma mkloc_add b i : mkloc b 0 +ₗ i = mkloc b i.
-Proof. rewrite /loc_add; cbn. by replace (0 + i)%Z with i%Z by lia. Qed.
+Lemma Loc_add b i : Loc b 0 +ₗ i = Loc b i.
+Proof. done. Qed.
 Definition fresh_block {X} (σ : gmap loc X) : block :=
   let loclst : list loc := elements (dom _ σ : gset loc) in
   let blockset : gset block := foldr (λ l, ({[loc_chunk l]} ∪.)) ∅ loclst in
   fresh blockset.
 
-Lemma is_fresh_block {X} (σ : gmap loc X) i : 
-  σ !! ({|loc_chunk := fresh_block σ; loc_idx := i |} : loc) = None.
+Lemma is_fresh_block {X} (σ : gmap loc X) i :
+  σ !! (Loc (fresh_block σ) i) = None.
 Proof.
   assert (∀ (l : loc) ls (S : gset block),
     l ∈ ls → (loc_chunk l) ∈ foldr (λ l, ({[(loc_chunk l)]} ∪.)) S ls) as help.
